\documentclass[a4paper]{article}

\usepackage[english]{babel}
\usepackage[utf8x]{inputenc}
\usepackage{amsmath}
\usepackage{graphicx}

\title{MATH 542 Homework 11}
\author{Saket Choudhary\\skchoudh@usc.edu}

\begin{document}
\maketitle

\section*{Problem 4b.1}
\begin{align*}
F &= \frac{n-p}{q}\frac{(Y-c1_n)'(P-P_H)(Y-c1_n)}{(Y-c1_n)'(I_n-P)(Y-c1_n)}\\
\end{align*}

Also, $X = \begin{pmatrix} 1 & x_{1,1} & x_{1,2} & \dots & x_{1,p-1}\\ 
1 & x_{2,1} & x_{2,2} & \dots & x_{2,p-1}\\
\vdots & \vdots & \vdots \\
1 & x_{n,1} & x_{n,2} & \dots & x_{n,p-1}\\
\end{pmatrix}$

Thus, $1_n \in \mathcal{C}(X)$ and hence $(I-P)1_n = 1_n'(I-P) = (P-P_H)1_n = 1_n'(P-P_H) = 0$ 
and hence $(Y-c1_n)'(P-P_H)(Y-c1_n) = Y'(P-P_H)Y-c1_n'(P-P_H)Y+cY'(P-P_H)1_n+c^21_n'(P-P_H)1_n = Y'(P-P_H)Y$

Similarly $(Y-c1_n)'(I-P)(Y-c1_n) = Y'(I-P)Y$
and hence $F$ statistic is the same as $F = \frac{n-p}{q}\frac{Y'(P-P_H)Y}{Y'(I_n-P)Y}$




\section*{Problem 4b.4}

\begin{align*}
\begin{pmatrix}
Y_1\\Y_2\\Y_3
\end{pmatrix} &= \begin{pmatrix}
1 & 1 \\
0 & 2 \\
-1 & 1\\
\end{pmatrix} \begin{pmatrix}\theta_1 \\ \theta_2 \end{pmatrix}+\begin{pmatrix}\epsilon_1\\ \epsilon_2\end{pmatrix}\\
&= X\beta+\epsilon\\
H:\ \theta_1 &= 2\theta_2\\
\implies \begin{pmatrix}1 & -2 \end{pmatrix}\\
&= A\beta = 0\\
F &= \frac{\frac{RSS_H-RSS}{q}}{\frac{RSS}{n-p}}\\
\end{align*}

Now,
\begin{align*}
\hat{\beta} &= (X'X)^{-1}X'Y\\
X'X = \begin{pmatrix} 2 & 0\\
0 & 6
\end{pmatrix}\\
(X'X)^{-1} &= \begin{pmatrix} 1/2 & 0\\
0 & 1/6
\end{pmatrix}\\
\hat{\beta} &= \begin{pmatrix} 1/2 & 0\\ 0 & 1/6 \end{pmatrix}\begin{pmatrix}\frac{Y_1-Y_3}{2}\\
\frac{Y_1+2Y_2+Y_3}{6}
\end{pmatrix}\\
\end{align*}

\begin{align*}
\hat{Y} &= X\hat{\beta}\\
&= \begin{pmatrix}
1 & 1 \\
0 & 2 \\
-1 & 1\\
\end{pmatrix}\begin{pmatrix}\frac{3Y_1-3Y_3}{6}\\
\frac{Y_1+2Y_2+Y_3}{6}
\end{pmatrix}\\
&= \begin{pmatrix}
\frac{4Y_1+2Y_2-2Y_3}{6}\\
\frac{Y_1+2Y_2+Y_3}{3}\\
\frac{-2Y_1+2Y_2+4Y_3}{6}\\
\end{pmatrix}
\end{align*}

\begin{align*}
RSS &= (Y-\hat{Y})'(Y-\hat{Y})\\
&= \begin{pmatrix}\frac{2Y_1-2Y_2+2Y_3}{6} &
\frac{-Y_1+Y_2-Y_3}{3} & \frac{2Y_1-2Y_2+2Y_3}{6}
\end{pmatrix}'.\begin{pmatrix}\frac{2Y_1-2Y_2+2Y_3}{6} \\
\frac{4y_1-4Y_2-2Y_3}{6} \\ \frac{2Y_1-2Y_2+2Y_3}{6}
\end{pmatrix}\\
&= \frac{1}{9}(Y_1-Y_2+Y_3)^2 + \frac{1}{9}(-Y_1+Y_2-Y_3)^2 + \frac{1}{9}(Y_1-Y_2+Y_3)^2\\
&= \frac{1}{3}(Y_1-Y_2+Y_3)^2
\end{align*}

\begin{align*}
A(X'X)^{-1}A' &= \begin{pmatrix}1/2 & -1/3 \end{pmatrix}\begin{pmatrix}
1 \\ -2
\end{pmatrix}\\
&= \frac{7}{6}\\
RSS_H-RSS &= [A\hat{\beta}]'[A(X'X)^{-1}A']^{-1}[A'\hat{\beta}]\\ 
&= \frac{6}{7}(\hat{\beta_1}-2\hat{\beta_2})^2
\end{align*}

Thus,
\begin{align*}
F &= \frac{\frac{6}{7}(\hat{\beta_1}-2\hat{\beta_2})^2}{\frac{1}{3}(Y_1-Y_2+Y_3)^2}
\end{align*}

\section*{Problem 4b.5}
$Y=I\theta+\epsilon$

$H: \theta_1 =\theta_3 $ or $\begin{pmatrix} 1 & 0 & -1 & 0 \end{pmatrix}\theta=0$

\begin{align*}
A &= \begin{pmatrix}
1 & 0 & -1 & 0
\end{pmatrix}\\
\hat{\beta} = \begin{pmatrix}
Y_1\\
Y_2\\
Y_3\\
Y_4
\end{pmatrix}\\
A\beta &= \begin{pmatrix} 1 & 0 & -1 & 0 \end{pmatrix} \begin{pmatrix}
Y_1\\Y_2\\Y_3\\Y_4
\end{pmatrix}\\
&= Y_1-Y_3\\
RSS_H-RSS &= \begin{pmatrix} Y_1 & -Y_3 \end{pmatrix}\frac{1}{2}\begin{pmatrix} Y_1 \\
-Y_3
\end{pmatrix}\\
&= \frac{1}{2}(Y_1-Y_3)^2\\
RSS = 3S^2\\
&= 3(Y_1+Y_2+Y_3+Y_4-0)^2\\
F &= \frac{RSS_H-RSS}{3S^2}\frac{3}{1}\\
&= \frac{(Y_1-Y_3)^2}{2(Y_1+Y_2+Y_3+Y_4)^2}
\end{align*}

\section*{Problem 4MISC.2}
\begin{align*}
\begin{pmatrix}
Y_{11}\\
Y_{12}\\
\vdots\\
Y_{1n}\\
Y_{21}\\
Y_{22}
\vdots\\
Y_{2n}
\end{pmatrix}&= \begin{pmatrix}x_1 & 0\\
x_2 & 0 \\
\vdots \\
x_n & 0\\
0 & x_1\\
0 & x_2\\
\vdots\\
0 & x_n
\end{pmatrix}\begin{pmatrix}\beta_1 \\ \beta_2\end{pmatrix} + \epsilon\\
H: A\hat{\beta} &=0 \implies \begin{pmatrix} 1 & -1 \end{pmatrix} = 0\\
A &= \begin{pmatrix} 1 & -1 \end{pmatrix}\\
X'X^{-1} &= \begin{pmatrix}\frac{1}{\sum_i x_i^2} & 0\\
0 & \frac{1}{\sum_i x_i^2}\end{pmatrix}\\
\hat{\beta} &= (X'X)^{-1}X'Y\\
&= \begin{pmatrix}\frac{1}{\sum_i x_i^2} & 0\\
0 & \frac{1}{\sum_i x_i^2}\end{pmatrix}  \begin{pmatrix}\sum_ix_i y_{i1}\\ \sum_i x_iy_{i2}\end{pmatrix}\\
&= \begin{pmatrix}\frac{\sum_ix_i y_{i1}}{\sum_i x_i^2}\\ \frac{\sum_i x_iy_{i2}}{\sum x_i^2}\end{pmatrix}\\
&= \begin{pmatrix}\hat{\beta_1} \\ \hat{\beta_2}\end{pmatrix}\\
RSS &= \sum_j\sum_i(y_{ji}-x_{ji}\beta_i)^2\\
&= \sum_i (y_{i1}^2-2y_{i1}x_i\hat{\beta_1} + x_{i1}^2\beta_1^2 + y_{i2}^2-2y_{2i}x_i + x_{2i}\beta_2^2)\\
RSS_H-RSS &= (A\beta)'[A'(X'X)^{-1}A]^{-1}(A\beta)\\
&= (\hat{\beta_1}-\hat{\beta_2}) [\begin{pmatrix} \frac{1}{\sum_i x_i^2} & \frac{-1}{\sum_i{x_i^2}} \end{pmatrix} \begin{pmatrix} 1\\ -1\end{pmatrix}]^{-1}\begin{pmatrix}\hat{\beta_1} \\ -\hat{\beta_2}\end{pmatrix}\\
&= (n-1)S^2
RSS_H-RSS &= (A\hat{\beta})'[A'(X'X)^{-1}A]^{-1}A\hat{\beta}\\
&= \frac{n}{n+1}(\bar{Y_n}-Y_{n+1})^2\\
&= \sum_i x_i^2 \frac{(\hat{\beta_1}-\hat{\beta_2})^2}{2}\\
F &= \frac{\frac{RSS_H-RSS}{1}}{\frac{(n-1)S^2}{n-1}}\\
&= \frac{\sum_i x_i^2\frac{(\beta_1-\beta_2)^2}{2}}{S^2}\\
&= \frac{(\beta_1-\beta_2)^2}{2S^2(\sum_x x_i^2)^{-1}}
\end{align*}

\section*{Problem 4MISC.4}
\begin{align*}
\begin{pmatrix} 
Y_1\\
Y_2\\
\vdots\\
Y_n\\
Y_{n+1}
\end{pmatrix}&= \begin{pmatrix}
1 & 0\\
1 & 0\\
\vdots & \vdots\\
1 & 0\\
0 & 1
\end{pmatrix}\begin{pmatrix}\mu_1 \\ \mu_2
\end{pmatrix}+ \begin{pmatrix} \epsilon_1\\
\epsilon_2\\
\vdots\\
\epsilon_n\\
\epsilon_{n+1}
\end{pmatrix}\\
H &:  A\hat{\beta} = 0 \implies \begin{pmatrix}1 & -1\end{pmatrix}\begin{pmatrix}\mu_1\\
\mu_2
\end{pmatrix} = 0 \\
X'X &= \begin{pmatrix}n & 0 \\ 0 & 1 \end{pmatrix}\\
(X'X)^{-1} &= \begin{pmatrix}1/n & 0 \\ 0 & 1 \end{pmatrix}\\
\begin{pmatrix}\hat{\mu_1}\\
\hat{\mu_2}
\end{pmatrix} &= \begin{pmatrix}\frac{1}{n}\sum_{i=1}^nY_i\\
Y_{n+1}
\end{pmatrix} = \begin{pmatrix} \bar{Y_n} \\ Y_{n+1}\end{pmatrix}\\ 
\begin{pmatrix} 
\hat{Y_1}\\
\hat{Y_2}\\
\vdots\\
\hat{Y_n}\\
\hat{Y_{n+1}}
\end{pmatrix}&= \begin{pmatrix} 
\bar{Y_n}\\
\bar{Y_2}\\
\vdots\\
\bar{Y_n}\\
\bar{Y_{n+1}}
\end{pmatrix}\\
RSS &= (Y-\hat{Y})'(Y-\hat{Y})\\
&= \begin{pmatrix}Y_1-\bar{Y_n} & Y_2-\bar{Y_n} & \dots Y_n-\bar{Y_n}& 0 \end{pmatrix}\begin{pmatrix}Y_1-\bar{Y_n} \\ Y_2-\bar{Y_n} \\ \vdots\\ Y_n-\bar{Y_n} \\ 0 \end{pmatrix}\\
&= \sum_{i=1}^n(Y_i-\bar{Y_n})^2\\
&= (n-1)S_n^2\\
F &= \frac{\frac{RSS_H-RSS}{1}}{\frac{RSS}{n+1-2}}\\
&= \frac{n}{n+1}\frac{(Y_{n+1}-\bar{Y_n})^2}{S_n^2}
\end{align*}

\end{document}