\documentclass[a4paper]{article}

\usepackage[english]{babel}
\usepackage[utf8x]{inputenc}
\usepackage{amsmath}
\usepackage{graphicx}

\title{MATH 542 Homework 4}
\author{Saket Choudhary\\skchoudh@usc.edu}

\begin{document}
\maketitle 
\section*{1a. Problem 1}

\begin{align*}
E[(X-a)(X-a)']&= E[(X-a)(X'-a')]\\
&= E[XX'-Xa'-aX'+aa']\\
&= E[XX']-E[Xa']-E[aX']+E[aa']\\
&= E[XX']-E[X]a'-aE[X']+E[aa']\\
&= (Var[X]+E[X]E[X]')-E[X]a'-aE[X']+aa'\\
&= Var[X]+ E[X]E[X]'-E[X]a'-aE[X]'+aa'\ \text{ since } E[X']=E[X]'\\
&= Var[X] + (E[X]-a)(E[X]'-a')\\
&= Var[X] + (E[X]-a)(E[X]-a)'
\end{align*}

$$Var[X] = \sum = (\sigma_{ij})$$

$$||X-a||_{1\times 1}^2 = (X-a)'_{1 \times r}(X-a)_{1 \times r}$$

And hence(replace $X$ with $X'$ and $a$ with $a'$):

\begin{align*}
E[||X-a||^2] &= E[(X-a)'(X-a)]\\
&= E[X'X]-E[X']a-a'E[X]+a'a\\
&= \sum_i E[X_i^2]-E[X']a-a'E[X]+a'a\\
&= \sum_i (Var[X_i]+E[X_i]^2)-E[X']a-a'E[X]+a'a\\
&= \sum_i Var[X_i]+ E[X']E[X]-E[X']a-a'E[X]+a'a\ \text{since } \sum_i E[X_i]^2 = E[X'X]\\
&=\sum_i Var[X_i]+ E[X]'E[X]-E[X]'a-a'E[X]+a'a\ \text{since } \sum_i E[X_i]^2 = E[X'X]\\
&= \sum_i Var[X_i] + (E[X]-a)'(E[X]-a)\\
&= \sum_i \sigma_i + ||E[X]-a||^2
\end{align*}

\section*{1a. Problem 2}
Fact: $X-a-E[X-a]=X-E[X]$
\begin{align*}
Cov[X-a,Y-b] &= E[(X-a-E[X-a])(Y-b-E[Y-b])'])\\
&= E[(X-E[X])(Y-E[Y])']\\
&= Cov[X,Y]
\end{align*}

\section*{1a. Problem 3}
$Y_i = X_i-X_{i-1}$

$Cov[Y_i,Y_j]=0$ for $i \neq j$

Consider the vector $(Y_1, Y_2, Y_3, \dots, Y_n)' = (X_1,X_2-X_1,X_3-X_2, \dots, X_n-X_{n-1})'$ 

We make use of $Var(AX) = AVar(X)A'$.

To find $A$, consider the vectors $(Y_1, Y_2, Y_3, \dots, Y_n)' = (X_1,X_2-X_1,X_3-X_2, \dots, X_n-X_{n-1})'$ 

\begin{align*}
\begin{pmatrix}
Y_1\\
Y_2\\
Y_3\\
\vdots\\
Y_n
\end{pmatrix} &= \begin{pmatrix}
X_1\\
X_2-X_1\\
X_3-X_2\\
\vdots\\
X_n-X_{n-1}
\end{pmatrix}\\
&= \begin{pmatrix}1 & 0 & 0 & \dots & 0 & 0\\
-1 & 1 & 0 & \dots & 0 & 0\\
0 & -1 & 1 & \dots & 0 & 0\\
\vdots & \vdots & \vdots & \vdots & \vdots & \vdots\\
0 & 0 & 0 & \dots & -1 & 1
\end{pmatrix} \times \begin{pmatrix}
X_1\\
X_2\\
X_3\\
\vdots\\
X_n
\end{pmatrix}
\end{align*}

Hence $A=\begin{pmatrix}1 & 0 & 0 & \dots & 0 & 0\\
-1 & 1 & 0 & \dots & 0 & 0\\
0 & -1 & 1 & \dots & 0 & 0\\
\vdots \\
0 & 0 & 0 & \dots & -1 & 1
\end{pmatrix}$


Now using $Var(Y) = AVar(X)A'$ we get 

$$Var(X) = A^{-1}Var(Y)A'^{-1}$$

$Var(Y) = I_{n\times n}$
and hence $Var(X) = A^{-1}A'^{-1} = BB^T$ where $B=A^{-1}$

\newpage 
\section*{Problem 4}

$X_{i+1} = \rho X_i$

Consider:

\begin{align*}
\begin{pmatrix}
X_1\\
X_2\\
X_3\\
\vdots\\
X_n
\end{pmatrix} &= \begin{pmatrix}
X_1\\
\rho X_1\\
\rho X_2\\
\vdots\\
\rho X_{n-1}
\end{pmatrix}\\
&= \begin{pmatrix}
1\\
\rho\\
\rho^2\\
\vdots\\
\rho^{n-1}
\end{pmatrix}X_1
\end{align*}

Let $A=\begin{pmatrix}1 & \rho & \rho^2 & \dots & \rho^{n-1}\end{pmatrix}'$
and hence variance $Var[X] = AVar(X_1)A' = \sigma^2AA'$

$Var[X] = \begin{pmatrix}
1 & \rho & \rho^2 & \dots & \rho^{n-1}\\
\rho & \rho^2 & \rho^3 & \dots & \rho^n\\
\rho^2 & \rho^3 & \rho^4 & \dots & \rho^{n+1}\\
\vdots & \vdots & \vdots & & \vdots\\
\rho^n & \rho^{n+1} & \rho^{n+2} & \dots & \rho^{2n-2}\\
\end{pmatrix}$

\section*{1b. Problem 1}

\begin{align*}
X_1^2+2X_1X_2-4X_2X_3+X_3^2 &= (X_1+X_2)X_1 + (X_1-2X_3)X_2 + (-2X_2+X_3)X_3\\
&= \begin{pmatrix}
X_1 & X_2 & X_2
\end{pmatrix}\begin{pmatrix}
1 & 1 & 0\\
1 & 0 & -2\\
0 & -2 & 1\\
\end{pmatrix}\begin{pmatrix}
X_1\\
X_2\\
X_3
\end{pmatrix}
\end{align*}

$$X=\begin{pmatrix}X_1 & X_2 & X_3\end{pmatrix}'$$

$$A = \begin{pmatrix}
1 & 1 & 0\\
1 & 0 & -2\\
0 & -2 & 1\\
\end{pmatrix}$$


$$A\sum = AVar[X] = \sigma^2\begin{pmatrix}
1 & 1 & \frac{1}{4}\\
1 & -\frac{1}{2} & -2\\
0 & -\frac{7}{4} & \frac{1}{2}\\
\end{pmatrix}$$


Thus, $$E[X'AX] = tr(A\sum) + \mu'A\mu = \sigma^2 + \mu'A\mu$$

\section*{1b. Problem 2}

\begin{align*}
\sum_i(X_i-\bar{X})^2 &= \sum_i (X_i^2-2X_i\bar{X}+\bar{X}^2)\\ 
&= \sum_i X_i^2 -2\sum_i X_i \bar{X} + \bar{X}^2\\  
&= \sum_i X_i^2 -n\bar{X}^2
\end{align*}

Now $\sum_iX_i^2 = X'X$ and $\bar{X} = \frac{1}{n}\sum_i X_i = \frac{1}{n} \mathbf{1'}X = \frac{1}{n}X'\mathbf{1} $

Hence,

\begin{align*}
\sum_i(X_i-\bar{X})^2 &= \sum_i X_i^2-n\bar{X}^2\\
&= X'X - n\frac{1}{n^2}(X'\mathbf{11'}X)\\
&= X'X-\frac{1}{n}(X'\mathbf{11'}X)\\
&= X'(\mathbf{I}-\frac{1}{n}\mathbf{11'})X
\end{align*}

Let $A=(\mathbf{I}-\frac{1}{n}\mathbf{11'})$

Now using $E[X'AX]= tr(A\sum) + \mu'A\mu$ we have:

\begin{align*}A\sum &= \begin{pmatrix}1-1/n & -1/n & -1/n & \dots & -1/n\\
-1/n & 1-1/n & -1/n & \dots & -1/n\\
\vdots\\
-1/n & -1/n & -1/n & \dots & 1-1/n
\end{pmatrix}\times diag(\sigma_1^2, \sigma_2^2, \dots, \sigma_n^2)\\ 
&= (1-\frac{1}{n})\sum_i \sigma_i^2
\end{align*}

Also, $$\mu'A = \begin{pmatrix} \mu & \mu & \dots & \mu \end{pmatrix} \times \begin{pmatrix}1-1/n & -1/n & -1/n & \dots & -1/n\\
-1/n & 1-1/n & -1/n & \dots & -1/n\\
\vdots\\
-1/n & -1/n & -1/n & \dots & 1-1/n
\end{pmatrix} = 0$$ 

and hence $\mu'A\mu=0$

\begin{align*}
E[\sum_i(X_i-\bar{X})^2] &= (1-\frac{1}{n})\sum_i \sigma_i^2  \\
E[\frac{1}{n(n-1)}\sum_i(X_i-\bar{X})^2]  &= \frac{1}{n^2} \sum_i \sigma_i^2
\end{align*}

Finally,

\begin{align*}
var(\bar{X}) &= Var(\frac{1}{n}\sum_i X_i)\\
&= \frac{1}{n^2} \sum_i Var(X_i)\\ \text{ since $X_i$ are mutually independent}\\
&= \frac{1}{n^2}\sum_i \sigma_i^2\\
&= E[\frac{1}{n(n-1)}\sum_i(X_i-\bar{X})^2]
\end{align*}

\section*{1b. Problem 3}

Given: $\bar{X_w} = \sum_i w_i X_i $ and $\sum w_i =1 $

\begin{align*}
Var(\bar{X_w}) &= Var(\sum w_i X_i)\\
&= \sum w_i^2Var(X_i)\ \text{ since $X_i$ are mutually independent}\\
&= \sum w_i^2 \sigma_i^2
\end{align*}

Now consider,

$$
\text{minimize} \sum w_i^2\sigma_i^2 \text{ subject to } \sum_i w_i =1
$$

We consider the following lagrange formulation:

$$min_w f(\mathbf{w}) = \sum_i w_i^2\sigma_i^2 +\lambda(\sum_iw_i-1)$$

Now to find optimal $\lambda$, we solve $\frac{\partial f(\mathbf{w})}{\partial w_i} = 0$

\begin{align*}
\frac{\partial f(\mathbf)}{\partial w_i} &= 2w_i\sigma_i^2+\lambda =0\\
\implies w_i &= -\frac{\lambda}{2\sigma_i^2}
\end{align*}

Thus, $w_i = -\frac{\lambda}{2\sigma_i^2}$ or $w_i \propto \frac{1}{\sigma_i^2}$

Using $\sum_i w_i=1$  we get:
\begin{eqnarray*}
\sum_i w_i = 1\\
\sum_i \frac{\lambda}{-2\sigma_i^2} =1\\
\implies \lambda = \frac{-2}{\sum_i 1/\sigma_i^2 }\\
\implies w_i = \frac{1}{\sigma_i^2 \sum_i(1/\sigma_i^2)}\\
\implies f_{min}(w) = \sum_i (\frac{1}{\sigma_i^2 \sum_i(1/\sigma_i^2)}) \sigma_i^2\\
v_{min} = \frac{1}{\sum_i(1/\sigma_i^2)}
\end{eqnarray*}


\subsection*{Part b}

\begin{align*}
\sum_i w_i (X_i-\bar{X_w})^2 &= \sum_i w_i(X_i^2-2X_i\bar{X_w}+\bar{X_w}^2)\\
&= \sum_i w_iX_i^2-2\bar{X_w}\sum_iw_iX_i+\bar{X_w^2}\\
&= \sum_i w_iX_i^2 -2\bar{X_w}^2+\bar{X_w}^2\\
&= \sum_i w_iX_i^2 -\bar{X_w}^2
\end{align*}

Now, we rewrite $\sum_i w_iX_i^2 = X'\Lambda X$ where $\Lambda = diag(w_1, w_2, \dots, w_n)$

and $\bar{X_w} = \sum_i w_iX_i = X'w = w'X$

\begin{align*}
\bar{X_w}^2 &= (\sum_i w_iX_i)^2\\
&=X'ww'X
\end{align*}

and hence $\sum_i w_i (X_i-\bar{X_w})^2=X'(\Lambda-ww')X$ 

Define $A=\Lambda-ww' = \begin{pmatrix}
w_1-w_1^2 & w_1w_2 & w_1w_3 & \dots & w_1w_n\\
w_2w_1 & w_2-w_2^2 & w_2w_3 & \dots & w_2w_n\\
\vdots & \vdots & \vdots & \vdots \\
w_nw_1 & w_nw_2 & w_nw_3 & \dots w_n-w_n^2\\
\end{pmatrix}$

so that 
$$E[\sum_i w_i (X_i-\bar{X_w})^2] = E[X'AX]= tr(A\sum) + \mu'A\mu$$


$$tr(A\sum) = \sum_i(w_i-w_i^2)\sigma_i^2 = \sum_i w_i\sigma_i^2-w_i(w_i\sigma_i^2) = \sum_i (a-aw_i) = na-a$$

and the $(1,1)$ element of the matrix $\mu'A$ is given by: 

\begin{align*}
\mu'A_1 &= \mu (w_1-w_1^2 - w_1\sum_{i=2}w_i)\\ &= w_1-w_1^2-w_1(1-w_1)\\ 
&= 0\end{align*}

and hence it's essentially a zero matrix(other elements are zero similarly)

Also, $$v_{min} = \frac{1}{\sum_i 1/\sigma_i^2} = \frac{1}{\sum_i \frac{w_i}{a}} = a$$

Thus,

\begin{align*}
E[S_w^2] &= \frac{1}{n-1} tr(A\sum) + \mu'A\mu\\
&= \frac{1}{n-1} (na-a) + 0\\
&=a\\
&= v_{min}
\end{align*}

\end{document}


